pcuic/theories/PCUICValidity.v
@@ -74,30 +74,36 @@ Section Validity.
     (lift_typing
         (fun (Σ0 : PCUICEnvironment.global_env_ext)
           (Γ0 : PCUICEnvironment.context) (_ T : term) =>
+          (* confluenv Σ0.1 -> *)
         isWfArity_or_Type Σ0 Γ0 T)).
   Proof.
     red. intros.
     red in X1 |- *.
-    destruct T. now eapply isWfArity_or_Type_extends.
+    destruct T. eapply isWfArity_or_Type_extends. all: eauto.
     destruct X1 as [s Hs]; exists s; now eapply isWfArity_or_Type_extends.
   Qed.
-  
+
   Theorem validity :
-    env_prop (fun Σ Γ t T => isWfArity_or_Type Σ Γ T)
+    env_prop (fun Σ Γ t T => confluenv Σ.1 -> isWfArity_or_Type Σ Γ T)
       (fun Σ Γ wfΓ =>
       All_local_env_over typing
-      (fun (Σ : global_env_ext) (Γ : context) (_ : wf_local Σ Γ) 
-         (t T : term) (_ : Σ;;; Γ |- t : T) => isWfArity_or_Type Σ Γ T) Σ Γ
+      (fun (Σ : global_env_ext) (Γ : context) (_ : wf_local Σ Γ)
+         (t T : term) (_ : Σ;;; Γ |- t : T) => confluenv Σ.1 -> isWfArity_or_Type Σ Γ T) Σ Γ
       wfΓ).
   Proof.
-    apply typing_ind_env; intros; rename_all_hyps.
+    apply typing_ind_env; intros (* ; rename_all_hyps *).
+    all: repeat match goal with
+    | h : confluenv _ -> _ |- _ =>
+      forward h by auto
+    end.
+    all: rename_all_hyps.
 
     - auto.
 
     - destruct (nth_error_All_local_env_over heq_nth_error X) as [HΓ' Hd].
       destruct decl as [na [b|] ty]; cbn -[skipn] in *.
       + destruct Hd as [Hd _].
-        eapply isWfArity_or_Type_lift; eauto. clear HΓ'. 
+        eapply isWfArity_or_Type_lift; eauto. clear HΓ'.
         now apply nth_error_Some_length in heq_nth_error.
       + destruct lookup_wf_local_decl; cbn -[skipn] in *.
         destruct o. right. exists x0. simpl in Hd.
@@ -183,15 +189,17 @@ Section Validity.
         apply inversion_Prod in Hu' as [na' [s1 [s2 Hs]]]; tas. intuition.
         eapply type_Cumul; pcuic.
         eapply (weakening_cumul Σ Γ [] [vass na A]) in b; pcuic.
-        simpl in b. eapply cumul_trans. auto. 2:eauto.
+        simpl in b. eapply cumul_trans. auto. auto. 2:eauto.
         constructor. constructor. simpl. apply leq_universe_product.
+
+    - admit.
 
     - destruct decl as [ty [b|] univs]; simpl in *.
       * eapply declared_constant_inv in X; eauto.
         red in X. simpl in X.
         eapply isWAT_weaken; eauto.
         eapply (isWAT_subst_instance_decl (Γ:=[])); eauto.
-        apply weaken_env_prop_isWAT.
+        (* apply weaken_env_prop_isWAT.
       * eapply isWAT_weaken; eauto.
         have ond := on_declared_constant _ _ _ wf H.
         do 2 red in ond. simpl in ond.
@@ -278,19 +286,20 @@ Section Validity.
       rewrite subst_instance_context_smash.
       rewrite (spine_subst_subst_to_extended_list_k sppar).
       assumption.
-      
+
     - (* Fix *)
       eapply nth_error_all in X0; eauto.
       firstorder auto.
-    
+
     - (* CoFix *)
       eapply nth_error_all in X0; eauto.
       firstorder auto.
 
     - (* Conv *)
       destruct X2. red in i. left. exact (projT1 i).
-      right. destruct s as [u [Hu _]]. now exists u.
-  Qed.
+      right. destruct s as [u [Hu _]]. now exists u. *)
+  (* Qed. *)
+  Admitted.
 
 End Validity.
 
@@ -298,7 +307,8 @@ Lemma validity_term {cf:checker_flags} {Σ Γ t T} :
   wf Σ.1 -> Σ ;;; Γ |- t : T -> isWfArity_or_Type Σ Γ T.
 Proof.
   intros. eapply validity; try eassumption.
-Defined.
+(* Defined. *)
+Admitted.
 
 (* This corollary relies strongly on validity.
    It should be used instead of the weaker [invert_type_mkApps],
@@ -310,7 +320,7 @@ Lemma inversion_mkApps :
     Σ ;;; Γ |- mkApps t l : T ->
     ∑ A, Σ ;;; Γ |- t : A × typing_spine Σ Γ A l T.
 Proof.
-  intros cf Σ Γ f u T wfΣ; induction u in f, T |- *. simpl. intros.
+  (* intros cf Σ Γ f u T wfΣ; induction u in f, T |- *. simpl. intros.
   { exists T. intuition pcuic. constructor. eapply validity; auto with pcuic.
     eauto. eapply cumul_refl'. }
   intros Hf. simpl in Hf.
@@ -327,5 +337,6 @@ Proof.
     econstructor. eapply validity; eauto with wf.
     eapply cumul_refl'. auto.
     clear -H'' HA''' wfΣ. depind H''.
-    econstructor; eauto. eapply cumul_trans; eauto.  
-Qed.
+    econstructor; eauto. eapply cumul_trans; eauto.
+Qed. *)
+Admitted.
